FOmegaC/Progress.v
@@ -1,0 +1,145 @@
+Require Import Coq.Lists.List.
+Require Export ParDB.Spec.
+Require Export ParDB.Lemmas.
+Require Export ParDB.Inst.
+
+Require Export SpecSyntax.
+Require Export SpecTyping.
+Require Export SpecEvaluation.
+Require Export LemmasTyping.
+Require Export Agreement.
+Require Export Consistency.
+
+Local Ltac crush :=
+  intros;
+  repeat
+    (cbn in *;
+     repeat crushSyntaxMatch;
+     repeat crushDbSyntaxMatchH;
+     repeat crushDbLemmasRewriteH;
+     repeat crushSyntaxRefold;
+     repeat crushTypingMatchH;
+     subst*;
+     try discriminate;
+     eauto with ws;
+     destruct_conjs;
+     idtac
+    ).
+
+Ltac canForm :=
+  repeat
+    (match goal with
+       | [H: ⟨ _ ⊢ _ : _ ~ _ ∷ _ ⟩ |- _] =>
+         eapply co_red in H
+       | [H: ⟨ _ ⊢ _ : arr _ _ ↝ _ ∷ _ ⟩ |- _] =>
+         inversion H; clear H
+       | [H: ⟨ _ ⊢ _ : arr _ _ ↝* _ ∷ _ ⟩ |- _] =>
+         eapply arr_consistency in H
+       | [H: ⟨ _ ⊢ _ : arrτ _ _ ↝* _ ∷ _ ⟩ |- _] =>
+         eapply arrτ_consistency in H
+       | [H: ⟨ _ ⊢ _ : arrγ _ _ _ _ ↝* _ ∷ _ ⟩ |- _] =>
+         eapply arrγ_consistency in H
+     end; crush); eauto 20 with ws.
+
+Lemma can_form_tarr' {t σ} (v: Value t) (wt: ⟨ nil ⊢ t : σ ⟩) :
+  ∀ γ τ1 τ2,
+    ⟨ nil ⊢ γ : σ ~ arr τ1 τ2 ∷ kstar ⟩ →
+    (∃ t' τ1', t = abs τ1' t') ∨
+    (∃ t' η τ1', t = cast (abs τ1' t') η).
+Proof.
+  depind wt; crush.
+  - canForm.
+  - canForm.
+  - inversion wt; clear wt; crush.
+    + pose proof (CoTrans nil H H0).
+      canForm.
+    + pose proof (CoTrans nil H H0).
+      canForm.
+Qed.
+
+Lemma can_form_arr {t σ1 σ2} (v: Value t) (wt: ⟨ nil ⊢ t : arr σ1 σ2 ⟩) :
+  (∃ t' τ', t = abs τ' t') ∨
+  (∃ t' γ τ', t = cast (abs τ' t') γ).
+Proof.
+  eapply (can_form_tarr' v wt).
+  eapply CoArr; eapply CoRefl;
+    eapply tm_agreement_ty in wt; crush.
+Qed.
+
+Lemma can_form_arrτ' {t σ} (v: Value t) (wt: ⟨ nil ⊢ t : σ ⟩) :
+  ∀ γ k τ,
+    ⟨ nil ⊢ γ : σ ~ arrτ k τ ∷ kstar ⟩ →
+    (∃ t', t = absτ k t') ∨
+    (∃ t' η, t = cast (absτ k t') η).
+Proof.
+  depind wt; crush.
+  - canForm.
+  - canForm.
+  - canForm.
+  - inversion wt; clear wt; crush.
+    + pose proof (CoTrans nil H H0).
+      canForm.
+    + pose proof (CoTrans nil H H0).
+      canForm.
+    + pose proof (CoTrans nil H H0).
+      canForm.
+Qed.
+
+Lemma can_form_arrτ {t k σ} (v: Value t) (wt: ⟨ nil ⊢ t : arrτ k σ ⟩) :
+  (∃ t', t = absτ k t') ∨
+  (∃ t' γ, t = cast (absτ k t') γ).
+Proof.
+  eapply (can_form_arrτ' v wt).
+  eapply CoArrτ; eapply CoRefl;
+    eapply tm_agreement_ty in wt; crush.
+Qed.
+
+
+Lemma can_form_arrγ' {t σ} (v: Value t) (wt: ⟨ nil ⊢ t : σ ⟩) :
+  ∀ γ k τ1 τ2 τ3,
+    ⟨ nil ⊢ γ : σ ~ arrγ τ1 τ2 k τ3 ∷ kstar ⟩ →
+    (∃ t' τ1' τ2', t = absγ τ1' τ2' k t') ∨
+    (∃ t' η τ1' τ2', t = cast (absγ τ1' τ2' k t') η).
+Proof.
+  depind wt; crush.
+  - canForm.
+  - canForm.
+  - canForm.
+  - inversion wt; clear wt; crush.
+    + pose proof (CoTrans nil H H0).
+      canForm.
+    + pose proof (CoTrans nil H H0).
+      canForm.
+    + pose proof (CoTrans nil H H0).
+      canForm.
+Qed.
+
+Lemma can_form_arrγ {t σ1 σ2 k σ3} (v: Value t) (wt: ⟨ nil ⊢ t : arrγ σ1 σ2 k σ3 ⟩) :
+  (∃ t' τ1' τ2', t = absγ τ1' τ2' k t') ∨
+  (∃ t' γ τ1' τ2', t = cast (absγ τ1' τ2' k t') γ).
+Proof.
+  eapply (can_form_arrγ' v wt).
+  eapply CoArrγ; eapply CoRefl;
+    eapply tm_agreement_ty in wt; crush.
+Qed.
+
+
+Ltac progressMatch :=
+  match goal with
+    | [ |- False ∨ _ ] => right
+    | [ |- True ∨ _ ] => left; trivial
+    | [ H: _ ∨ _ |- _ ] => destruct H
+    | [ vt: Value ?t, wt: ⟨ nil ⊢ ?t : arr _ _ ⟩ |- _ ] =>
+      apply (can_form_arr vt) in wt
+    | [ vt: Value ?t, wt: ⟨ nil ⊢ ?t : arrτ _ _ ⟩ |- _ ] =>
+      apply (can_form_arrτ vt) in wt
+    | [ vt: Value ?t, wt: ⟨ nil ⊢ ?t : arrγ _ _ _ _ ⟩ |- _ ] =>
+      apply (can_form_arrγ vt) in wt
+  end.
+
+Lemma progress {t σ} (wt: ⟨ nil ⊢ t : σ ⟩) :
+  Value t ∨ ∃ t', t --> t'.
+Proof with destruct_conjs; subst*; eauto using eval.
+  depind wt; intuition; crush; repeat progressMatch; crush; eauto using eval.
+  - inversion wt; crush; eauto using eval.
+Qed.
